Abort ExampleSimpleMem proof

src/ExampleSimpleMem.v
@@ -1,20 +1,10 @@
 From sflib Require Import sflib.
 From Paco Require Import paco.
 Require Import Coq.Classes.RelationClasses Lia Program.
-From Fairness Require Export ITreeLib WFLib FairBeh NatStructs Mod pind OpenMod SCM.
+From Fairness Require Export ITreeLib WFLib FairBeh NatStructs Mod pind OpenMod SCM Red IRed.
 
 Set Implicit Arguments.
 
-
-Definition call {R} {ID E} `{@eventE ID -< E} `{OpenMod.callE -< E} {A} (fn: string) (arg: A): itree E R :=
-  r <- trigger (OpenMod.Call fn arg↑);;
-  unwrap (r↓)
-.
-
-Definition callR R {ID E} `{@eventE ID -< E} `{OpenMod.callE -< E} {A} (fn: string) (arg: A): itree E R :=
-  r <- trigger (OpenMod.Call fn arg↑);;
-  unwrap (r↓)
-.
 
 Section MOD.
   Definition loc_l: SCMem.val := SCMem.val_ptr (0, 0).
@@ -23,14 +13,14 @@ Section MOD.
   Definition example_fun:
     ktree ((((@eventE void) +' cE) +' (sE unit)) +' OpenMod.callE) unit unit :=
     fun _ =>
-      b <- call "cas" (loc_l, SCMem.val_nat 0, SCMem.val_nat 1);;
+      b <- OMod.call "cas" (loc_l, SCMem.val_nat 0, SCMem.val_nat 1);;
       if (b: bool) then
-        call "store" (loc_f, SCMem.val_nat 1)
+        OMod.call "store" (loc_f, SCMem.val_nat 1)
       else
         ITree.iter
           (fun _ =>
-             f <- call "load" loc_f;;
-             b <- call "compare" (f: SCMem.val, SCMem.val_nat 1);;
+             f <- OMod.call "load" loc_f;;
+             b <- OMod.call "compare" (f: SCMem.val, SCMem.val_nat 1);;
              if (b: bool) then Ret (inr tt) else Ret (inl tt)) tt
   .
 
@@ -117,17 +107,19 @@ Section SIM.
   Qed.
 
   Let I_aux (w: W): iProp :=
+        (∃ ths, own_threads_white ths)
+          **
         (∃ m,
             (memory_black m)
               **
               (OwnM (Auth.white (Excl.just (tt, m): @Excl.t _): stateTgtRA (unit * SCMem.t)%type)))
           **
-          (∃ im_tgt,
-              (OwnM (Auth.white (Excl.just im_tgt: @Excl.t (imap thread_id nat_wf)): identThsRA))
+          (∃ im_ths,
+              (OwnM (Auth.white (Excl.just im_ths: @Excl.t (imap thread_id nat_wf)): identThsRA))
                 **
                 (match w with
                  | W_bot => points_to loc_l (SCMem.val_nat 0) ** points_to loc_f (SCMem.val_nat 0) ** (OwnM (Excl.just tt: @URA.car (Excl.t unit)))
-                 | W_own th k o i => points_to loc_l (SCMem.val_nat 1) ** points_to loc_f (SCMem.val_nat 0) ** ⌜im_tgt th <= i⌝ ** own_thread th ** monoWhite k ge_PreOrder o
+                 | W_own th k o i => points_to loc_l (SCMem.val_nat 1) ** points_to loc_f (SCMem.val_nat 0) ** ⌜im_ths th <= i⌝ ** own_thread th ** monoWhite k ge_PreOrder o
                  | W_top => points_to loc_l (SCMem.val_nat 1) ** points_to loc_f (SCMem.val_nat 1) ** (OwnM (Excl.just tt: @URA.car (Excl.t unit)))
                  end))
   .
@@ -319,19 +311,51 @@ Section SIM.
   (*       ⌜fair_update im_tgt0 im_tgt1 (sum_fmap_l (tids_fmap tid ths))⌝ *)
   (*       -* *)
 
-  Lemma close_itree_trigger_call2
-        omd md
-        R
-        fn args ktr
-    :
-    @OMod.close_itree omd md R (trigger (OpenMod.Call fn args) >>= ktr) = UB.
-      (* match (md.(Mod.funs) fn) with *)
-      (* | Some body => *)
-      (*     trigger (Yield);;; rv <- OMod.embed_itree omd md (body args);; tau;; OMod.close_itree omd md (ktr rv) *)
-      (* | None => Vis ((embed_event_l Undefined|)|)%sum (Empty_set_rect _) *)
-      (* end. *)
-  Proof.
-  Admitted.
+  (* Ltac _red_close_itree f := *)
+  (*   match goal with *)
+  (*   | [ |- ITree.bind (OMod.close_itree _ _ ?itr) _ = _ ] => *)
+  (*       match itr with *)
+  (*       | ITree.bind _ _ => *)
+  (*           instantiate (f:=_continue); eapply interp_tgt_bind; fail *)
+  (*       | Tau _ => *)
+  (*           instantiate (f:=_break); apply interp_tgt_tau; fail *)
+  (*       | Ret _ => *)
+  (*           instantiate (f:=_continue); apply interp_tgt_ret; fail *)
+  (*       | trigger ?e => *)
+  (*           instantiate (f:=_break); *)
+  (*           match (type of e) with *)
+  (*           | context[hCallE] => apply interp_tgt_hcall *)
+  (*           | context[eventE] => apply interp_tgt_triggere *)
+  (*           | context[pE] => apply interp_tgt_triggerp *)
+  (*           | _ => fail 2 *)
+  (*           end *)
+  (*       | triggerUB => *)
+  (*           instantiate (f:=_break); apply interp_tgt_triggerUB; fail *)
+  (*       | triggerNB => *)
+  (*           instantiate (f:=_break); apply interp_tgt_triggerNB; fail *)
+  (*       | unwrapU _ => *)
+  (*           instantiate (f:=_break); apply interp_tgt_unwrapU; fail *)
+  (*       | unwrapN _ => *)
+  (*           instantiate (f:=_break); apply interp_tgt_unwrapN; fail *)
+  (*       | assume _ => *)
+  (*           instantiate (f:=_break); apply interp_tgt_assume; fail *)
+  (*       | guarantee _ => *)
+  (*           instantiate (f:=_break); apply interp_tgt_guarantee; fail *)
+  (*       | _ => *)
+  (*           fail *)
+  (*       end *)
+  (*   | [ |- interp_hCallE_tgt _ _ _ _ = _] => *)
+  (*       instantiate (f:=_continue); apply bind_ret_r_rev; fail *)
+  (*   | _ => fail *)
+  (*   end. *)
+
+  (* Ltac _red_lsim f := *)
+  (*   _red_interp_tgt f || _red_itree f || fail. *)
+
+  (* Ltac ired_l := try (prw _red_lsim 2 1 0). *)
+  (* Ltac ired_r := try (prw _red_lsim 1 1 0). *)
+
+  (* Ltac ired_both := ired_l; ired_r. *)
 
   (*       isim tid I r g Q itr_src itr_tgt ths im_src im_tgt1 st_src st_tgt. *)
 
@@ -341,225 +365,325 @@ Section SIM.
     { econs. exact 0. }
     { i. exists (S o0). ss. }
     { cut (forall tid,
-              own_thread tid ⊢ stsim I tid itop5 itop5 (fun r_src r_tgt => I ** own_thread tid ** ⌜r_src = r_tgt⌝) (example_spec_fun tt) (OMod.close_itree (example_omod) (SCMem.mod [1; 1]) (example_fun tt))).
+              I ** own_thread tid ⊢ stsim I tid itop5 itop5 (fun r_src r_tgt => I ** own_thread tid ** ⌜r_src = r_tgt⌝) (example_spec_fun tt) (OMod.close_itree (example_omod) (SCMem.mod [1; 1]) (example_fun tt))).
       { admit. }
-      i. iIntros "TID". ss. unfold example_spec_fun, example_fun.
-      unfold ExampleSimpleMem.call at 1.
-      rewrite ! close_itree_bind. ired.
+      i. iIntros "[INV TID]". ss. unfold example_spec_fun, example_fun.
 
-      match goal with
-      | >>=
+      repeat (prw _red_itree 1 2 0).
 
-      set (@close_itree_trigger_call2
-                 example_omod (SCMem.mod [1; 1])
-                 _
-                 "cas" (Any.upcast (loc_l, SCMem.val_nat 0, SCMem.val_nat 1))
-                 (fun r: Any.t => (` x : bool <-
-                                          OMod.close_itree example_omod (SCMem.mod [1; 1]) (unwrap (Any.downcast r));;
-                                        OMod.close_itree example_omod (SCMem.mod [1; 1])
-                                                         (if x
-                                                          then ExampleSimpleMem.call "store" (loc_f, SCMem.val_nat 1)
-                                                          else
-                                                            ITree.iter
-                                                              (λ _ : (),
-                                                                  ` f : SCMem.val <- ExampleSimpleMem.call "load" loc_f;;
-                                                                        ` b : bool <- ExampleSimpleMem.call "compare" (f, SCMem.val_nat 1);;
-                                                                              (if b then Ret (inr ()) else Ret (inl ()))) ())): itree (((eventE +' cE) +' sE (OMod.state example_omod)) +' OpenMod.callE) Any.t)).
+      rewrite ! close_itree_bind. rewrite close_itree_call. ss.
+      repeat (prw _red_itree 1 1 0).
+      iApply (stsim_yieldR with "INV"). iIntros "INV".
 
-                 setoid_rewrite close_itree_trigger_call.
-
-      rewrite ! close_itree_bind. ired.
-      rewrite close_itree_trigger_call.
-
-
-      unfold call.
+      iDestruct "INV" as (w) "[MONO [[[% THS] MEM] [% [TMAP INV]]]]".
+      iExists _, _. iSplitL "TMAP"; [auto|]. iSplit; [auto|]. iIntros (im_ths1) "% TMAP".
+      repeat (prw _red_itree 1 1 0).
 
 
 
+      unfold Mod.wrap_fun. rewrite Any.upcast_downcast.
+      unfold SCMem.cas_fun. ss.
 
-@isim_gen tid itop10 itop10 _ _ (fun r_src r_tgt ths im_src im_tgt st_src st_tgt =>
-                                                                  I ths im_src im_tgt st_src st_tgt
-                                                                    ** own_thread tid
-                                                                    ** ⌜r_src = r_tgt⌝)%I example_fun_spec example_fun).
+      rewrite ! embed_itree_bind.
+      repeat (prw _red_itree 1 1 0).
+      rewrite embed_itree_ret.
+      repeat (prw _red_itree 1 1 0).
+      rewrite ! embed_itree_bind.
+      repeat (prw _red_itree 1 1 0).
 
+      rewrite ! embed_itree_trigger_get2.
+      repeat (prw _red_itree 1 1 0).
 
-instantiate (1:=fun ths im_src im_tgt st_src st_tgt => (default_I ths im_src im_tgt st_src st_tgt ** I)%I).
+      iDestruct "MEM" as "[% [MEM MOWN]]".
 
-liftI I). admit. }
-    i. ss.
+      iApply stsim_getR. iSplit.
+      { iFrame. }
+      repeat (prw _red_itree 1 1 0).
+      iApply stsim_tauR.
+      repeat (prw _red_itree 1 1 0).
+      ss.
 
-    cut (forall tid,
-            own_thread tid ⊢ @isim_gen tid itop10 itop10 _ _ (fun r_src r_tgt ths im_src im_tgt st_src st_tgt =>
-                                                                I ths im_src im_tgt st_src st_tgt
-                                                                  ** own_thread tid
-                                                                  ** ⌜r_src = r_tgt⌝)%I example_fun_spec example_fun).
-    { admit. }
-
-    unfold example_fun_spec, example_fun.
-    unfold isim_gen. i. iIntros "TID".
-    iIntros (ths im_src im_tgt0 st_src st_tgt im_tgt1) "INV %".
-    iDestruct "INV" as "[THS INV]". iDestruct "INV" as (w) "[MONO INV]".
-    destruct w.
-
-    3:{
-      unfold I_aux. des_ifs.
-      iPoseProof (black_persistent_white with "MONO") as "#WHITE".
-      iDestruct "INV" as "[% OWN]". des. subst.
-      iApply isim_getR.
-      ired. rewrite unfold_iter_eq. ired.
-
-      admit.
-
-      (* iApply isim_yieldR. iFrame. *)
-      (* iIntros (? ? ? ? ? ?) "INV %". *)
-      (* iPoseProof (I_fair_update with "TID INV") as "[TID INV]"; eauto. *)
+(*       rewrite embed_itree_ret. *)
+(*       repeat (prw _red_itree 1 1 0). *)
+(*       rewrite ! embed_itree_bind. *)
+(*       repeat (prw _red_itree 1 1 0). *)
 
 
-      (* iApply isim_getR. ired. iApply isim_sync. *)
-      (* iSplitR "TID". *)
-      (* { unfold I. iFrame. iExists W_top. iFrame. auto. } *)
-      (* iIntros (ths1 im_src1 im_tgt2 st_src1 st_tgt1 im_tgt3) "INV". *)
-      (* iIntros. iApply isim_ret. *)
-      (* iPoseProof (I_fair_update with "TID INV") as "[TID INV]"; eauto. *)
-      (* iFrame. auto. *)
-    }
 
-    1:{
-      iPoseProof (black_persistent_white with "MONO") as "#WHITE".
-      unfold I_aux. des_ifs. iDestruct "INV" as "[% OWN]". subst.
-      iApply isim_getR.
+(*  with "INV"). iIntros "INV". *)
 
-      iDestruct (monoBlack_alloc ge_PreOrder 6) as "-# > [%k ORD]".
-      iPoseProof (black_updatable with "MONO") as "> MONO".
-      { instantiate (1:=W_own tid k 6 (im_tgt1 (inl tid))). econs. }
-      iClear "WHITE".
-      iPoseProof (black_persistent_white with "MONO") as "#WHITE".
 
-      iApply isim_putR.
+(*       rewrite ! embed_itree_bind. *)
 
-      iApply isim_yieldR.
-      iPoseProof (black_persistent_white with "ORD") as "# -# ORDWHITE".
-      iSplitR "OWN ORD".
-      { unfold I. iFrame. iExists (W_own _ _ _ _). iFrame.
-        iSplit; auto.
-      }
-      iIntros (? ? ? ? ? ?) "INV %".
 
-      iPoseProof (I_stutter with "WHITE OWN INV ORD") as "> [[OWN INV] ORD]".
-      { eapply Nat.lt_succ_diag_r. }
-      iApply isim_yieldR. iFrame.
-      iIntros (? ? ? ? ? ?) "INV %".
+(*       rewrite ! embed_itree_bind. *)
 
-      iPoseProof (locked_after_own with "WHITE INV") as "%".
-      destruct st_tgt0. ss. subst.
-      iApply isim_getR.
 
-      iPoseProof (I_stutter with "WHITE OWN INV ORD") as "> [[OWN INV] ORD]".
-      { eapply Nat.lt_succ_diag_r. }
-      iApply isim_yieldR. iFrame.
-      iIntros (? ? ? ? ? ?) "INV %".
+(*       rewrite ! close_itree_bind. rewrite close_itree_call. ss. *)
+(*       repeat (prw _red_itree 1 1 0). *)
+(*       iApply (stsim_yieldR with "INV"). iIntros "INV". *)
 
-      iPoseProof (I_stutter with "WHITE OWN INV ORD") as "> [[OWN INV] ORD]".
-      { eapply Nat.lt_succ_diag_r. }
-      iApply isim_yieldR. iFrame.
-      iIntros (? ? ? ? ? ?) "INV %".
 
-      iApply isim_putR.
-      iPoseProof (I_finish with "WHITE OWN INV") as "> [[INV TID] TOP]".
+(* { *)
 
-      iApply isim_yieldR. iFrame.
-      iIntros (? ? ? ? ? ?) "INV %".
-      iPoseProof (I_fair_update with "TID INV") as "[TID INV]"; eauto.
+(* iFrame. iSplit. *)
+(*       { *)
 
-      iApply isim_sync. iFrame.
-      iIntros (? ? ? ? ? ?) "INV %".
-      iPoseProof (I_fair_update with "TID INV") as "[TID INV]"; eauto.
 
-      iApply isim_ret. iFrame. auto.
-    }
+(*       rewrite ! close_itree_bind. rewrite close_itree_call. ss. *)
 
-    {
-      iPoseProof (black_persistent_white with "MONO") as "#WHITE".
-      unfold I_aux. des_ifs. iDestruct "INV" as "[[% OWN] MONOWHITE]". des. subst.
-      iApply isim_getR.
 
-      iStopProof.
-      revert ths im_src st_src im_tgt0 im_tgt1 b0 th H1 H.
-      pattern o, i. match goal with | |- ?f o i => change (f (fst (o, i)) (snd (o, i))) end.
-      generalize (o, i) as oi. clear o i. intros oi.
+(* ired. *)
 
-      induction (prod_lt_well_founded Nat.lt_wf_0 Nat.lt_wf_0 oi). clear H. rename H0 into IH.
-      i. destruct x as [o i]. subst.
-      iIntros "[WHITE [TID [THS [MONO [OWN MONOWHITE]]]]]".
 
-      iPoseProof (thread_disjoint with "TID OWN") as "%".
-      iPoseProof (black_updatable with "MONO") as "> MONO".
-      { ss. instantiate (1:= W_own th k o (im_tgt1 (inl th))). econs.
-        specialize (H (inl th)).
-        unfold sum_fmap_l, tids_fmap in H. des_ifs.
-        { ss. lia. }
-        { lia. }
-      }
-      iClear "WHITE".
-      iPoseProof (black_persistent_white with "MONO") as "#WHITE".
+(*       ired. *)
 
-      rewrite unfold_iter_eq. ired.
+(*       unfold ExampleSimpleMem.call at 1. *)
+(*       rewrite ! close_itree_bind. ired. *)
+(*       rewrite close_itree_trigger_call2. ss. *)
 
-      admit.
+(*       repeat (prw _red_itree 1 1 0). *)
 
-      (* iApply isim_getR. destruct b0. *)
-      (* { ired. *)
-      (*   iApply isim_sync. *)
-      (*   iSplitR "TID". *)
-      (*   { unfold I. iFrame. iExists (W_own _ _ _ _). iFrame. iPureIntro. auto. } *)
-      (*   iIntros (ths1 im_src1 im_tgt2 st_src1 st_tgt1 im_tgt3) "INV". *)
-      (*   iIntros. iApply isim_ret. iSplitL; auto. *)
-      (*   iPoseProof (I_fair_update with "TID INV") as "[TID INV]"; eauto. *)
-      (*   iFrame. *)
-      (* } *)
-      (* { ired. iPoseProof (threads_in with "THS OWN") as "%". *)
-      (*   iApply isim_yieldR. *)
-      (*   { iSplitR "TID". *)
-      (*     { unfold I. iFrame. iExists (W_own _ _ _ _). iFrame. iPureIntro. auto. } *)
-      (*     iIntros (ths1 im_src1 im_tgt2 st_src1 st_tgt1 im_tgt3) "INV". *)
-      (*     iIntros. iApply isim_tauR. *)
-      (*     iDestruct "INV" as "[THS INV]". iDestruct "INV" as (w) "[MONO INV]". *)
-      (*     destruct st_tgt1 as [l f]. ss. *)
-      (*     iPoseProof (black_white_compare with "WHITE MONO") as "%". *)
-      (*     inv H4. *)
-      (*     { guardH LE. iDestruct "INV" as "[[% OWN] MONOWHITE]". des. subst. *)
-      (*       iPoseProof (threads_in with "THS OWN") as "%". *)
-      (*       iApply IH. *)
-      (*       3:{ eauto. } *)
-      (*       2:{ instantiate (1:=(o0, _)). simpl. eauto. } *)
-      (*       { inv LE. *)
-      (*         { left. auto. } *)
-      (*         { des. right. *)
-      (*           { lia. } *)
-      (*           { cut (im_tgt1 (inl th) < im_tgt0 (inl th)). *)
-      (*             { lia. } *)
-      (*             specialize (H (inl th)). unfold sum_fmap_l, tids_fmap in H. *)
-      (*             des_ifs. *)
-      (*           } *)
-      (*         } *)
-      (*       } *)
-      (*       iClear "WHITE". *)
-      (*       iPoseProof (black_persistent_white with "MONO") as "#WHITE". *)
-      (*       iFrame. auto. *)
-      (*     } *)
-      (*     { iDestruct "INV" as "[% INV]". des. subst. *)
-      (*       rewrite unfold_iter_eq. ired. *)
-      (*       iApply isim_getR. ired. *)
-      (*       iApply isim_sync. iSplitR "TID". *)
-      (*       { unfold I. iFrame. iExists W_top. iFrame. auto. } *)
-      (*       { iIntros (? ? ? ? ? ?) "INV %". *)
-      (*         iApply isim_ret. *)
-      (*         iPoseProof (I_fair_update with "TID INV") as "[TID INV]"; eauto. *)
-      (*         iFrame. auto. *)
-      (*       } *)
-      (*     } *)
-      (*   } *)
-      (* } *)
-    }
+(*       eapply _einit. *)
+(*       { eapply f_equal. eapply f_equal. *)
+(*         eapply close_itree_trigger_call2. *)
+(*         Set Printing All. *)
+
+
+(* Ltac _ctx n := *)
+(*   match n with *)
+(*   | O => apply f_equal *)
+(*   | S ?m => apply _equal_f; _ctx m *)
+(*   end. *)
+
+(*       Ltac _tmp f := instantiate (f:=_break); eapply close_itree_trigger_call. *)
+(*       prw _tmp 1 1 0. *)
+
+
+(*       pose (OMod.close_itree example_omod (SCMem.mod [1; 1]) *)
+(*         (trigger *)
+(*            (OpenMod.Call "cas" (Any.upcast (loc_l, SCMem.val_nat 0, SCMem.val_nat 1))))). *)
+
+(*       Ltac aaa := *)
+
+(*       prw (l *)
+
+(*       repeat (prw _red_gen 1 1 0). *)
+(*       repeat (prw _red_gen 1 2 0). *)
+
+(*       match goal with *)
+(*       | >>= *)
+
+(*       set (@close_itree_trigger_call2 *)
+(*                  example_omod (SCMem.mod [1; 1]) *)
+(*                  _ *)
+(*                  "cas" (Any.upcast (loc_l, SCMem.val_nat 0, SCMem.val_nat 1)) *)
+(*                  (fun r: Any.t => (` x : bool <- *)
+(*                                           OMod.close_itree example_omod (SCMem.mod [1; 1]) (unwrap (Any.downcast r));; *)
+(*                                         OMod.close_itree example_omod (SCMem.mod [1; 1]) *)
+(*                                                          (if x *)
+(*                                                           then ExampleSimpleMem.call "store" (loc_f, SCMem.val_nat 1) *)
+(*                                                           else *)
+(*                                                             ITree.iter *)
+(*                                                               (λ _ : (), *)
+(*                                                                   ` f : SCMem.val <- ExampleSimpleMem.call "load" loc_f;; *)
+(*                                                                         ` b : bool <- ExampleSimpleMem.call "compare" (f, SCMem.val_nat 1);; *)
+(*                                                                               (if b then Ret (inr ()) else Ret (inl ()))) ())): itree (((eventE +' cE) +' sE (OMod.state example_omod)) +' OpenMod.callE) Any.t)). *)
+
+(*                  setoid_rewrite close_itree_trigger_call. *)
+
+(*       rewrite ! close_itree_bind. ired. *)
+(*       rewrite close_itree_trigger_call. *)
+
+
+(*       unfold call. *)
+
+
+
+
+(* @isim_gen tid itop10 itop10 _ _ (fun r_src r_tgt ths im_src im_tgt st_src st_tgt => *)
+(*                                                                   I ths im_src im_tgt st_src st_tgt *)
+(*                                                                     ** own_thread tid *)
+(*                                                                     ** ⌜r_src = r_tgt⌝)%I example_fun_spec example_fun). *)
+
+
+(* instantiate (1:=fun ths im_src im_tgt st_src st_tgt => (default_I ths im_src im_tgt st_src st_tgt ** I)%I). *)
+
+(* liftI I). admit. } *)
+(*     i. ss. *)
+
+(*     cut (forall tid, *)
+(*             own_thread tid ⊢ @isim_gen tid itop10 itop10 _ _ (fun r_src r_tgt ths im_src im_tgt st_src st_tgt => *)
+(*                                                                 I ths im_src im_tgt st_src st_tgt *)
+(*                                                                   ** own_thread tid *)
+(*                                                                   ** ⌜r_src = r_tgt⌝)%I example_fun_spec example_fun). *)
+(*     { admit. } *)
+
+(*     unfold example_fun_spec, example_fun. *)
+(*     unfold isim_gen. i. iIntros "TID". *)
+(*     iIntros (ths im_src im_tgt0 st_src st_tgt im_tgt1) "INV %". *)
+(*     iDestruct "INV" as "[THS INV]". iDestruct "INV" as (w) "[MONO INV]". *)
+(*     destruct w. *)
+
+(*     3:{ *)
+(*       unfold I_aux. des_ifs. *)
+(*       iPoseProof (black_persistent_white with "MONO") as "#WHITE". *)
+(*       iDestruct "INV" as "[% OWN]". des. subst. *)
+(*       iApply isim_getR. *)
+(*       ired. rewrite unfold_iter_eq. ired. *)
+
+(*       admit. *)
+
+(*       (* iApply isim_yieldR. iFrame. *) *)
+(*       (* iIntros (? ? ? ? ? ?) "INV %". *) *)
+(*       (* iPoseProof (I_fair_update with "TID INV") as "[TID INV]"; eauto. *) *)
+
+
+(*       (* iApply isim_getR. ired. iApply isim_sync. *) *)
+(*       (* iSplitR "TID". *) *)
+(*       (* { unfold I. iFrame. iExists W_top. iFrame. auto. } *) *)
+(*       (* iIntros (ths1 im_src1 im_tgt2 st_src1 st_tgt1 im_tgt3) "INV". *) *)
+(*       (* iIntros. iApply isim_ret. *) *)
+(*       (* iPoseProof (I_fair_update with "TID INV") as "[TID INV]"; eauto. *) *)
+(*       (* iFrame. auto. *) *)
+(*     } *)
+
+(*     1:{ *)
+(*       iPoseProof (black_persistent_white with "MONO") as "#WHITE". *)
+(*       unfold I_aux. des_ifs. iDestruct "INV" as "[% OWN]". subst. *)
+(*       iApply isim_getR. *)
+
+(*       iDestruct (monoBlack_alloc ge_PreOrder 6) as "-# > [%k ORD]". *)
+(*       iPoseProof (black_updatable with "MONO") as "> MONO". *)
+(*       { instantiate (1:=W_own tid k 6 (im_tgt1 (inl tid))). econs. } *)
+(*       iClear "WHITE". *)
+(*       iPoseProof (black_persistent_white with "MONO") as "#WHITE". *)
+
+(*       iApply isim_putR. *)
+
+(*       iApply isim_yieldR. *)
+(*       iPoseProof (black_persistent_white with "ORD") as "# -# ORDWHITE". *)
+(*       iSplitR "OWN ORD". *)
+(*       { unfold I. iFrame. iExists (W_own _ _ _ _). iFrame. *)
+(*         iSplit; auto. *)
+(*       } *)
+(*       iIntros (? ? ? ? ? ?) "INV %". *)
+
+(*       iPoseProof (I_stutter with "WHITE OWN INV ORD") as "> [[OWN INV] ORD]". *)
+(*       { eapply Nat.lt_succ_diag_r. } *)
+(*       iApply isim_yieldR. iFrame. *)
+(*       iIntros (? ? ? ? ? ?) "INV %". *)
+
+(*       iPoseProof (locked_after_own with "WHITE INV") as "%". *)
+(*       destruct st_tgt0. ss. subst. *)
+(*       iApply isim_getR. *)
+
+(*       iPoseProof (I_stutter with "WHITE OWN INV ORD") as "> [[OWN INV] ORD]". *)
+(*       { eapply Nat.lt_succ_diag_r. } *)
+(*       iApply isim_yieldR. iFrame. *)
+(*       iIntros (? ? ? ? ? ?) "INV %". *)
+
+(*       iPoseProof (I_stutter with "WHITE OWN INV ORD") as "> [[OWN INV] ORD]". *)
+(*       { eapply Nat.lt_succ_diag_r. } *)
+(*       iApply isim_yieldR. iFrame. *)
+(*       iIntros (? ? ? ? ? ?) "INV %". *)
+
+(*       iApply isim_putR. *)
+(*       iPoseProof (I_finish with "WHITE OWN INV") as "> [[INV TID] TOP]". *)
+
+(*       iApply isim_yieldR. iFrame. *)
+(*       iIntros (? ? ? ? ? ?) "INV %". *)
+(*       iPoseProof (I_fair_update with "TID INV") as "[TID INV]"; eauto. *)
+
+(*       iApply isim_sync. iFrame. *)
+(*       iIntros (? ? ? ? ? ?) "INV %". *)
+(*       iPoseProof (I_fair_update with "TID INV") as "[TID INV]"; eauto. *)
+
+(*       iApply isim_ret. iFrame. auto. *)
+(*     } *)
+
+(*     { *)
+(*       iPoseProof (black_persistent_white with "MONO") as "#WHITE". *)
+(*       unfold I_aux. des_ifs. iDestruct "INV" as "[[% OWN] MONOWHITE]". des. subst. *)
+(*       iApply isim_getR. *)
+
+(*       iStopProof. *)
+(*       revert ths im_src st_src im_tgt0 im_tgt1 b0 th H1 H. *)
+(*       pattern o, i. match goal with | |- ?f o i => change (f (fst (o, i)) (snd (o, i))) end. *)
+(*       generalize (o, i) as oi. clear o i. intros oi. *)
+
+(*       induction (prod_lt_well_founded Nat.lt_wf_0 Nat.lt_wf_0 oi). clear H. rename H0 into IH. *)
+(*       i. destruct x as [o i]. subst. *)
+(*       iIntros "[WHITE [TID [THS [MONO [OWN MONOWHITE]]]]]". *)
+
+(*       iPoseProof (thread_disjoint with "TID OWN") as "%". *)
+(*       iPoseProof (black_updatable with "MONO") as "> MONO". *)
+(*       { ss. instantiate (1:= W_own th k o (im_tgt1 (inl th))). econs. *)
+(*         specialize (H (inl th)). *)
+(*         unfold sum_fmap_l, tids_fmap in H. des_ifs. *)
+(*         { ss. lia. } *)
+(*         { lia. } *)
+(*       } *)
+(*       iClear "WHITE". *)
+(*       iPoseProof (black_persistent_white with "MONO") as "#WHITE". *)
+
+(*       rewrite unfold_iter_eq. ired. *)
+
+    (*   admit. *)
+
+    (*   (* iApply isim_getR. destruct b0. *) *)
+    (*   (* { ired. *) *)
+    (*   (*   iApply isim_sync. *) *)
+    (*   (*   iSplitR "TID". *) *)
+    (*   (*   { unfold I. iFrame. iExists (W_own _ _ _ _). iFrame. iPureIntro. auto. } *) *)
+    (*   (*   iIntros (ths1 im_src1 im_tgt2 st_src1 st_tgt1 im_tgt3) "INV". *) *)
+    (*   (*   iIntros. iApply isim_ret. iSplitL; auto. *) *)
+    (*   (*   iPoseProof (I_fair_update with "TID INV") as "[TID INV]"; eauto. *) *)
+    (*   (*   iFrame. *) *)
+    (*   (* } *) *)
+    (*   (* { ired. iPoseProof (threads_in with "THS OWN") as "%". *) *)
+    (*   (*   iApply isim_yieldR. *) *)
+    (*   (*   { iSplitR "TID". *) *)
+    (*   (*     { unfold I. iFrame. iExists (W_own _ _ _ _). iFrame. iPureIntro. auto. } *) *)
+    (*   (*     iIntros (ths1 im_src1 im_tgt2 st_src1 st_tgt1 im_tgt3) "INV". *) *)
+    (*   (*     iIntros. iApply isim_tauR. *) *)
+    (*   (*     iDestruct "INV" as "[THS INV]". iDestruct "INV" as (w) "[MONO INV]". *) *)
+    (*   (*     destruct st_tgt1 as [l f]. ss. *) *)
+    (*   (*     iPoseProof (black_white_compare with "WHITE MONO") as "%". *) *)
+    (*   (*     inv H4. *) *)
+    (*   (*     { guardH LE. iDestruct "INV" as "[[% OWN] MONOWHITE]". des. subst. *) *)
+    (*   (*       iPoseProof (threads_in with "THS OWN") as "%". *) *)
+    (*   (*       iApply IH. *) *)
+    (*   (*       3:{ eauto. } *) *)
+    (*   (*       2:{ instantiate (1:=(o0, _)). simpl. eauto. } *) *)
+    (*   (*       { inv LE. *) *)
+    (*   (*         { left. auto. } *) *)
+    (*   (*         { des. right. *) *)
+    (*   (*           { lia. } *) *)
+    (*   (*           { cut (im_tgt1 (inl th) < im_tgt0 (inl th)). *) *)
+    (*   (*             { lia. } *) *)
+    (*   (*             specialize (H (inl th)). unfold sum_fmap_l, tids_fmap in H. *) *)
+    (*   (*             des_ifs. *) *)
+    (*   (*           } *) *)
+    (*   (*         } *) *)
+    (*   (*       } *) *)
+    (*   (*       iClear "WHITE". *) *)
+    (*   (*       iPoseProof (black_persistent_white with "MONO") as "#WHITE". *) *)
+    (*   (*       iFrame. auto. *) *)
+    (*   (*     } *) *)
+    (*   (*     { iDestruct "INV" as "[% INV]". des. subst. *) *)
+    (*   (*       rewrite unfold_iter_eq. ired. *) *)
+    (*   (*       iApply isim_getR. ired. *) *)
+    (*   (*       iApply isim_sync. iSplitR "TID". *) *)
+    (*   (*       { unfold I. iFrame. iExists W_top. iFrame. auto. } *) *)
+    (*   (*       { iIntros (? ? ? ? ? ?) "INV %". *) *)
+    (*   (*         iApply isim_ret. *) *)
+    (*   (*         iPoseProof (I_fair_update with "TID INV") as "[TID INV]"; eauto. *) *)
+    (*   (*         iFrame. auto. *) *)
+    (*   (*       } *) *)
+    (*   (*     } *) *)
+    (*   (*   } *) *)
+    (*   (* } *) *)
+    (* } *)
   Admitted.
 End SIM.
